Splinter/Paged/PagedSystemRefinement.i.dfy
@@ -1,0 +1,501 @@
+include "PagedSystem.i.dfy"
+
+// This module shows refinement of CoordinatorMod to
+// CrashTolerantMapSpecMod, thereby functioning as the top layer in a
+// refinement stack for program models in refinement layers below.
+
+// TODO(jonh): satisfy a refinement-module proof obligation!
+module PagedSystemRefinement(journalMod: JournalIfc) {
+  import opened SequencesLite // Last, DropLast
+  import opened CM = CoordinatorMod(journalMod)
+  import opened StampedMapMod
+  import opened MsgHistoryMod
+  import opened KeyType
+  import opened ValueMessage
+  import opened FullKMMapMod
+  import MapSpecMod
+  import opened JM = journalMod
+
+  import Async = CrashTolerantMapSpecMod.async
+  type Journal = MsgHistory
+
+  function EphemeralSeqEnd(ephemeral: Ephemeral) : LSN
+    requires ephemeral.WF() && ephemeral.Known?
+  {
+    IEJ(ephemeral.journal).SeqEndFor(ephemeral.mapadt.seqEnd)
+  }
+
+  function StampedMapToVersion(sm: StampedMapMod.StampedMap) : CrashTolerantMapSpecMod.Version
+  {
+    CrashTolerantMapSpecMod.Version(Async.PersistentState(MapSpecMod.Variables(sm.mi)))
+  }
+
+  function VersionsWithForgottenPrefix(base: StampedMapMod.StampedMap, msgHistory: MsgHistory, stableLSN: LSN) : (versions:seq<CrashTolerantMapSpecMod.Version>)
+    requires msgHistory.WF()
+    requires msgHistory.CanFollow(base.seqEnd)
+    requires msgHistory.CanDiscardTo(stableLSN)
+    ensures |versions| == msgHistory.SeqEndFor(base.seqEnd)+1
+  {
+    // Construct a Version seq with the entries before stableLSN Forgotten: that's what spec expects.
+    var numVersions := msgHistory.SeqEndFor(base.seqEnd) + 1;
+    seq(numVersions, lsn requires 0<=lsn<numVersions =>
+      if lsn < stableLSN
+      then CrashTolerantMapSpecMod.Forgotten
+      else StampedMapToVersion(MapPlusHistory(base, msgHistory.DiscardRecent(lsn))))
+  }
+
+  function I(v: Variables) : CrashTolerantMapSpecMod.Variables
+  {
+    if !Inv(v)
+    then CrashTolerantMapSpecMod.InitState()  // silly-handler
+    else
+      var stableLSN := v.persistentImage.SeqEnd();
+      if v.ephemeral.Known?
+      then CrashTolerantMapSpecMod.Variables(
+        VersionsWithForgottenPrefix(v.persistentImage.mapadt, IEJ(v.ephemeral.journal), stableLSN),
+          v.ephemeral.progress, v.ephemeral.syncReqs, stableLSN)
+      else CrashTolerantMapSpecMod.Variables(
+        VersionsWithForgottenPrefix(v.persistentImage.mapadt, IPJ(v.persistentImage.journal), stableLSN),
+          Async.InitEphemeralState(), map[], stableLSN)
+  }
+
+  // Where these journals share an LSN, they map it to the same message.
+  predicate JournalOverlapsAgree(j0: Journal, j1: Journal)
+    requires j0.WF() && j1.WF()
+  {
+    forall lsn | j0.Contains(lsn) && j1.Contains(lsn) :: j0.msgs[lsn] == j1.msgs[lsn]
+  }
+
+  predicate JournalExtendsJournal(jlong: Journal, jshort: Journal, startLsn: LSN)
+    requires jlong.WF() && jshort.WF()
+    requires jlong.CanFollow(startLsn)
+    requires jshort.CanFollow(startLsn)
+  {
+    && jlong.CanDiscardTo(jshort.SeqEndFor(startLsn))            // jlong is longer
+    && jlong.DiscardRecent(jshort.SeqEndFor(startLsn)) == jshort // they agree on contents in overlap
+  }
+
+  predicate InvPersistentJournalGeometry(v: Variables)
+    requires v.WF()
+  {
+    && IPJ(v.persistentImage.journal).CanFollow(v.persistentImage.mapadt.seqEnd)
+  }
+
+  predicate InvEphemeralGeometry(v: Variables)
+    requires v.WF() && v.ephemeral.Known?
+  {
+    // Ephemeral journal begins at persistent map
+    && IEJ(v.ephemeral.journal).CanFollow(v.persistentImage.mapadt.seqEnd)
+    // Ephemeral map ends no earlier than persistent map
+    && v.persistentImage.mapadt.seqEnd <= v.ephemeral.mapadt.seqEnd
+    // Ephemeral journal ends no earlier than ephmeral map
+    // (With the first conjunct, this conjunct happens to subsume the second conjunct,
+    // but this was the nicest way to write it.)
+    && IEJ(v.ephemeral.journal).CanDiscardTo(v.ephemeral.mapadt.seqEnd)
+    // Ephemeral journal is no shorter than persistent state
+    && v.persistentImage.SeqEnd() <= EphemeralSeqEnd(v.ephemeral)
+  }
+
+  predicate InvEphemeralValueAgreement(v: Variables)
+    requires v.WF() && v.ephemeral.Known?
+    requires InvEphemeralGeometry(v)
+  {
+    // Ephemeral journal agrees with persistent journal
+    && JournalOverlapsAgree(IPJ(v.persistentImage.journal), IEJ(v.ephemeral.journal))
+    // Ephemeral map state agrees with ephemeral journal (tacked onto persistent map)
+    && v.ephemeral.mapadt == MapPlusHistory(v.persistentImage.mapadt, IEJ(v.ephemeral.journal).DiscardRecent(v.ephemeral.mapadt.seqEnd))
+  }
+
+  predicate InvFrozenGeometry(v: Variables)
+    requires v.WF() && v.ephemeral.Known?
+    requires v.ephemeral.frozenMap.Some?
+  {
+    // frozen map hsan't passed ephemeral journal
+    && v.ephemeral.frozenMap.value.seqEnd <= EphemeralSeqEnd(v.ephemeral)
+  }
+
+  predicate FrozenMapDoesntRegress(v: Variables)
+  {
+    && v.ephemeral.Known?
+    && v.ephemeral.frozenMap.Some?
+    // And it doesn't stop before the persistent image map (so we'll be able
+    // to DiscardOld on the ephemeral journal to see they agree)
+    && v.persistentImage.mapadt.seqEnd <= v.ephemeral.frozenMap.value.seqEnd
+  }
+
+  predicate InvFrozenValueAgreement(v: Variables)
+    requires v.WF()
+    requires v.ephemeral.Known?
+    requires InvEphemeralGeometry(v)
+    requires v.ephemeral.frozenMap.Some?
+    requires InvFrozenGeometry(v)
+  {
+    // Agreement is only defined when FrozenMapDoesntRegress, but
+    // FrozenMapDoesntRegress isn't an invariant because we runtime-check it at
+    // the moment we need it, in CommitStart.
+    FrozenMapDoesntRegress(v) ==>
+      v.ephemeral.frozenMap.value == MapPlusHistory(v.persistentImage.mapadt, IEJ(v.ephemeral.journal).DiscardRecent(v.ephemeral.frozenMap.value.seqEnd))
+    // NB: Frozen Journal agreement comes "for free" because the frozen
+    // journal is just defined as the frozenJournalLSN prefix of the
+    // ephemeral journal.
+  }
+
+  predicate InvInFlightGeometry(v: Variables)
+    requires v.WF() && v.inFlightImage.Some?
+  {
+    && var ifImage := v.inFlightImage.value;
+
+    // We need a well-behaved journal to relate in-flight state to.
+    && v.ephemeral.Known?
+    && InvEphemeralGeometry(v)
+
+    // Geometry properties
+    // In-flight map + journal stitch.
+    && IPJ(ifImage.journal).CanFollow(ifImage.mapadt.seqEnd)
+    // Commiting in-flight state won't shrink persistent state
+    && v.persistentImage.SeqEnd() <= ifImage.SeqEnd()
+    // In-flight map doesn't precede persistent map -- that would cause
+    // forgotten lsns to pop back into existence, and we don't have those lsns
+    // in the ephemeral journal to compare to.
+    && v.persistentImage.mapadt.seqEnd <= ifImage.mapadt.seqEnd
+    // in-flight view hsan't passed ephemeral journal
+    && ifImage.SeqEnd() <= EphemeralSeqEnd(v.ephemeral)
+  }
+
+  predicate InvInFlightValueAgreement(v: Variables)
+    requires v.WF() && v.inFlightImage.Some?
+    requires InvInFlightGeometry(v)
+  {
+    && var ifImage := v.inFlightImage.value;
+    // in-flight journal is consistent with the persistent journal
+    && JournalOverlapsAgree(IPJ(ifImage.journal), IPJ(v.persistentImage.journal))
+    // in-flight journal is consistent with the ephemeral journal
+    && JournalOverlapsAgree(IPJ(ifImage.journal), IEJ(v.ephemeral.journal))
+    // in-flight map matches corresponding state in ephemeral world
+    && ifImage.mapadt == MapPlusHistory(v.persistentImage.mapadt,
+                      IEJ(v.ephemeral.journal).DiscardRecent(ifImage.mapadt.seqEnd))
+  }
+
+  predicate Inv(v: Variables)
+  {
+    && v.WF()
+    && InvPersistentJournalGeometry(v)
+    && (v.ephemeral.Known? ==>
+      && InvEphemeralGeometry(v)
+      && InvEphemeralValueAgreement(v)
+
+      && (v.ephemeral.frozenMap.Some? ==>
+        && InvFrozenGeometry(v)
+        && InvFrozenValueAgreement(v)
+        )
+      )
+    && (v.inFlightImage.Some? ==>
+      && InvInFlightGeometry(v)
+      && InvInFlightValueAgreement(v)
+      )
+  }
+
+  lemma InitRefines(v: Variables)
+    requires v.Mkfs()
+    ensures Inv(v)
+    ensures I(v) == CrashTolerantMapSpecMod.InitState()
+  {
+    assert I(v).versions[0].asyncState.appv.kmmap == FullKMMapMod.EmptyKMMap(); // trigger
+  }
+
+  lemma CommitStepPreservesHistory(v: Variables, v': Variables, uiop: UIOp, step: Step, lsn: LSN)
+    requires Inv(v)
+    requires Next(v, v', uiop)
+    requires NextStep(v, v', uiop, step);
+    requires step.CommitCompleteStep?
+    requires v.persistentImage.mapadt.seqEnd <= lsn <= EphemeralSeqEnd(v.ephemeral)
+    requires v.inFlightImage.value.mapadt.seqEnd <= lsn  // Can't do much with lsns that have been forgotten
+    ensures IEJ(v'.ephemeral.journal).CanDiscardTo(lsn);
+    ensures MapPlusHistory(v.persistentImage.mapadt, IEJ(v.ephemeral.journal).DiscardRecent(lsn))
+            == MapPlusHistory(v'.persistentImage.mapadt, IEJ(v'.ephemeral.journal).DiscardRecent(lsn));
+  {
+    // There are six pieces in play here: the persistent and in-flight images and the ephemeral journals:
+    //  _________ __________
+    // | pdi.map | pdi.jrnl |
+    //  --------- ----------
+    //  ______________R__________
+    // | idi.map      | idi.jrnl |
+    //  -------------- ----------
+    //            ____________________
+    //           | eph.jrnl           |
+    //            --------------------
+    //                 _______________
+    //                | eph'.jrnl     |
+    //                 ---------------
+    // "R" is the "reference LSN" -- that's where we're going to prune ephemeral.journal, since
+    // after the commit it is going to be the LSN of the persistent map.
+
+    var refLsn := v.inFlightImage.value.mapadt.seqEnd;
+    var ej := IEJ(v.ephemeral.journal);
+    var eji := ej.DiscardRecent(lsn);
+
+    // Here's a calc, but in comments so we can use a shorthand algebra:
+    // Let + represent both MapPlusHistory and Concat (they're associative).
+    // Let [x..] represent DiscardOld(x) and [..y] represent DiscardRecent(y).
+    // var im:=v.inFlightImage.value.mapadt, pm:=v.persistentImage.mapadt, R:=im.seqEnd
+    // pm'+ej'[..lsn]
+    // im+ej'[..lsn]
+    // im+ej[..lsn][R..]
+    //   {InvInFlightVersionAgreement}
+    // (pm+ej[..R])+ej[..lsn][R..]
+    JournalAssociativity(v.persistentImage.mapadt, ej.DiscardRecent(refLsn), ej.DiscardRecent(lsn).DiscardOld(refLsn));
+    // pm+(ej[..R]+ej[..lsn][R..])
+    assert ej.DiscardRecent(refLsn) == ej.DiscardRecent(lsn).DiscardRecent(refLsn);  // because R <= lsn; smaller lsn are Forgotten
+    // pm+(ej[..lsn][..R]+ej[..lsn][R..])
+    assert eji.DiscardRecent(refLsn).Concat(eji.DiscardOld(refLsn)) == eji;  // trigger
+    // pm+ej[..lsn]
+  }
+
+  lemma {:timeLimitMultiplier 2} InvInductivePutStep(v: Variables, v': Variables, uiop: UIOp, step: Step)
+    requires Inv(v)
+    requires Next(v, v', uiop)
+    requires NextStep(v, v', uiop, step)
+    requires step.PutStep?
+    ensures Inv(v')
+  {
+    if v.inFlightImage.Some? {
+      var idiEnd := v.inFlightImage.value.mapadt.seqEnd;
+      assert IEJ(v.ephemeral.journal).DiscardRecent(idiEnd) == IEJ(v'.ephemeral.journal).DiscardRecent(idiEnd); // trigger
+    }
+    if FrozenMapDoesntRegress(v') {
+      assert FrozenMapDoesntRegress(v);
+      var frozenEnd := v.ephemeral.frozenMap.value.seqEnd;
+      assert IEJ(v.ephemeral.journal).DiscardRecent(frozenEnd) == IEJ(v'.ephemeral.journal).DiscardRecent(frozenEnd); // trigger
+      assert v'.ephemeral.frozenMap.value == MapPlusHistory(v'.persistentImage.mapadt, IEJ(v'.ephemeral.journal).DiscardRecent(v'.ephemeral.frozenMap.value.seqEnd));
+      assert InvFrozenValueAgreement(v');
+    }
+
+    // InvEphemeralMapIsJournalSnapshot
+    var key := uiop.baseOp.req.input.key;
+    var val := uiop.baseOp.req.input.value;
+    var singleton := MsgHistoryMod.Singleton(NextLSN(v), KeyedMessage(key, Define(val)));
+    JournalAssociativity(v.persistentImage.mapadt, IEJ(v.ephemeral.journal), singleton);
+    assert IEJ(v.ephemeral.journal).DiscardRecent(v.ephemeral.mapadt.seqEnd) == IEJ(v.ephemeral.journal); // trigger
+    assert IEJ(v'.ephemeral.journal) == IEJ(v'.ephemeral.journal).DiscardRecent(v'.ephemeral.mapadt.seqEnd); // trigger
+    // TODO(chris): I'm wondering why these subexpressions aren't sort of
+    // self-triggering? It's a very common pattern in this code.
+//    calc {
+//      v'.ephemeral.mapadt;
+//      MapPlusHistory(v.ephemeral.mapadt, singleton);
+//      MapPlusHistory(MapPlusHistory(v.persistentImage.mapadt, v.ephemeral.journal.DiscardRecent(v.ephemeral.mapadt.seqEnd)), singleton);
+//      MapPlusHistory(MapPlusHistory(v.persistentImage.mapadt, v.ephemeral.journal), singleton);
+//      MapPlusHistory(v.persistentImage.mapadt, v.ephemeral.journal.Concat(singleton));
+//      MapPlusHistory(v.persistentImage.mapadt, v'.ephemeral.journal);
+//      MapPlusHistory(v'.persistentImage.mapadt, v'.ephemeral.journal.DiscardRecent(v'.ephemeral.mapadt.seqEnd));
+//    }
+    assert Inv(v');
+  }
+
+  lemma InvInductiveCommitCompleteStep(v: Variables, v': Variables, uiop: UIOp, step: Step)
+    requires Inv(v)
+    requires Next(v, v', uiop)
+    requires NextStep(v, v', uiop, step)
+    requires step.CommitCompleteStep?
+    ensures Inv(v')
+  {
+    if FrozenMapDoesntRegress(v') {
+      assert FrozenMapDoesntRegress(v);
+      calc {
+        v'.ephemeral.frozenMap.value;
+        v.ephemeral.frozenMap.value;
+        MapPlusHistory(v.persistentImage.mapadt, IEJ(v.ephemeral.journal).DiscardRecent(v.ephemeral.frozenMap.value.seqEnd));
+        {
+          CommitStepPreservesHistory(v, v', uiop, step, v.ephemeral.frozenMap.value.seqEnd);
+        }
+        MapPlusHistory(v'.persistentImage.mapadt, IEJ(v'.ephemeral.journal).DiscardRecent(v'.ephemeral.frozenMap.value.seqEnd));
+      }
+    }
+
+    // InvEphemeralMapIsJournalSnapshot
+    var pm := v.persistentImage.mapadt;
+    var em := v.ephemeral.mapadt;
+    var ej := IEJ(v.ephemeral.journal);
+    var imEnd := v.inFlightImage.value.mapadt.seqEnd;
+
+    JournalAssociativity(pm, ej.DiscardRecent(imEnd), ej.DiscardOld(imEnd).DiscardRecent(em.seqEnd));
+    assert ej.DiscardRecent(em.seqEnd) == ej.DiscardRecent(imEnd).Concat(ej.DiscardOld(imEnd).DiscardRecent(em.seqEnd));   // trigger
+  }
+
+  lemma InvInductive(v: Variables, v': Variables, uiop: UIOp)
+    requires Inv(v)
+    requires Next(v, v', uiop)
+    ensures Inv(v')
+  {
+    var step :| NextStep(v, v', uiop, step);
+    match step {
+      case LoadEphemeralFromPersistentStep() => {
+        assert Inv(v');
+      }
+      case RecoverStep(puts) => {
+        // InvEphemeralMapIsJournalSnapshot
+        var em := v.ephemeral.mapadt;
+        var ej := v.ephemeral.journal;
+        JournalAssociativity(v.persistentImage.mapadt, IEJ(ej).DiscardRecent(em.seqEnd), puts);
+        assert IEJ(ej).DiscardRecent(em.seqEnd).Concat(puts)
+          == IEJ(v'.ephemeral.journal).DiscardRecent(v'.ephemeral.mapadt.seqEnd);  // trigger
+      }
+      case AcceptRequestStep() => {
+        assert Inv(v');
+      }
+      case QueryStep() => {
+        assert Inv(v');
+      }
+      case PutStep() => {
+        InvInductivePutStep(v, v', uiop, step);
+      }
+      case DeliverReplyStep() => {
+        assert Inv(v');
+      }
+//    case JournalInternalStep(sk) => { assert Inv(v'); }
+//    case SplinterTreeInternalStep(sk) => { assert Inv(v'); }
+      case ReqSyncStep() => {
+        assert Inv(v');
+      }
+      case ReplySyncStep() => {
+        assert Inv(v');
+      }
+      case FreezeMapAdtStep() => {
+        assert v'.ephemeral.Known?;
+        assert v'.ephemeral.frozenMap.Some?;
+        calc {
+          v'.ephemeral.frozenMap.value;
+          MapPlusHistory(v'.persistentImage.mapadt, IEJ(v'.ephemeral.journal).DiscardRecent(v'.ephemeral.frozenMap.value.seqEnd));
+        }
+        assert InvFrozenValueAgreement(v');
+        assert Inv(v');
+      }
+      case CommitStartStep(seqBoundary) => {
+        assert Inv(v');
+      }
+      case CommitCompleteStep() => {
+        InvInductiveCommitCompleteStep(v, v', uiop, step);
+      }
+      case CrashStep() => {
+        assert Inv(v');
+      }
+    }
+  }
+
+  lemma {:timeLimitMultiplier 2} JournalAssociativity(x: MapAdt, y: Journal, z: Journal)
+    requires y.WF()
+    requires z.WF()
+    requires y.CanFollow(x.seqEnd)
+    requires z.CanFollow(y.SeqEndFor(x.seqEnd))
+    ensures MapPlusHistory(MapPlusHistory(x, y), z) == MapPlusHistory(x, y.Concat(z))
+    decreases z.Len();
+  {
+    if !z.EmptyHistory? {
+      var ztrim := z.DiscardRecent(z.seqEnd - 1);
+      var yz := y.Concat(z);
+
+      JournalAssociativity(x, y, ztrim);
+      assert yz.DiscardRecent(yz.seqEnd - 1) == y.Concat(ztrim); // trigger
+    }
+  }
+
+  lemma {:timeLimitMultiplier 4} PutStepRefines(v: Variables, v': Variables, uiop: UIOp, step: Step)
+    requires Inv(v)
+    requires Next(v, v', uiop)
+    requires NextStep(v, v', uiop, step);
+    requires step.PutStep?
+    ensures Inv(v')
+    ensures CrashTolerantMapSpecMod.Next(I(v), I(v'), uiop)
+  {
+    InvInductivePutStep(v, v', uiop, step);
+
+    var j := IEJ(v.ephemeral.journal);
+    var j' := IEJ(v'.ephemeral.journal);
+    var base := v.persistentImage.mapadt;
+    var key := uiop.baseOp.req.input.key;
+    var value := uiop.baseOp.req.input.value;
+
+    assert j'.MsgHistory? ==> j' == j'.DiscardRecent(j'.Len() + j'.seqStart);  // seq trigger
+    assert j.MsgHistory? ==> j == j.DiscardRecent(j.Len() + j.seqStart);  // seq trigger
+
+    assert forall i | v.persistentImage.mapadt.seqEnd<=i<|I(v).versions| :: j'.DiscardRecent(i) == j.DiscardRecent(i);  // Rob Power Trigger
+
+    assert CrashTolerantMapSpecMod.NextStep(I(v), I(v'), uiop); // witness
+  }
+
+  lemma CommitStepRefines(v: Variables, v': Variables, uiop: UIOp, step: Step)
+    requires Inv(v)
+    requires Next(v, v', uiop)
+    requires NextStep(v, v', uiop, step);
+    requires step.CommitCompleteStep?
+    ensures Inv(v')
+    ensures CrashTolerantMapSpecMod.Next(I(v), I(v'), uiop)
+  {
+    // See description & diagram in CommitStepPreservesHistory.
+    InvInductive(v, v', uiop);
+    forall i | 0<=i<|I(v).versions|
+      ensures I(v').versions[i] == if i < I(v').stableIdx then CrashTolerantMapSpecMod.Forgotten else I(v).versions[i]
+    {
+      if v.inFlightImage.value.SeqEnd() <= i {
+        CommitStepPreservesHistory(v, v', uiop, step, i);
+      }
+    }
+    assert CrashTolerantMapSpecMod.NextStep(I(v), I(v'), UIOp.SyncOp);  // witness
+  }
+
+  lemma {:timeLimitMultiplier 2} NextRefines(v: Variables, v': Variables, uiop: UIOp)
+    requires Inv(v)
+    requires Next(v, v', uiop)
+    ensures Inv(v')
+    ensures CrashTolerantMapSpecMod.Next(I(v), I(v'), uiop)
+  {
+    InvInductive(v, v', uiop);
+
+    var step :| NextStep(v, v', uiop, step);
+    match step {
+      case LoadEphemeralFromPersistentStep() => {
+        assert uiop == CrashTolerantMapSpecMod.NoopOp;
+        assert CrashTolerantMapSpecMod.NextStep(I(v), I(v'), uiop); // case boilerplate
+      }
+      case RecoverStep(puts) => {
+        assert uiop == CrashTolerantMapSpecMod.NoopOp;
+        assert CrashTolerantMapSpecMod.NextStep(I(v), I(v'), uiop); // case boilerplate
+      }
+      case AcceptRequestStep() => {
+        assert CrashTolerantMapSpecMod.NextStep(I(v), I(v'), uiop); // case boilerplate
+      }
+      case QueryStep() => {
+        assert CrashTolerantMapSpecMod.NextStep(I(v), I(v'), uiop); // case boilerplate
+      }
+      case PutStep() => {
+        PutStepRefines(v, v', uiop, step);
+      }
+      case DeliverReplyStep() => {
+        assert CrashTolerantMapSpecMod.NextStep(I(v), I(v'), uiop); // case boilerplate
+      }
+//    case JournalInternalStep(sk) => { assert Inv(v'); }
+//    case SplinterTreeInternalStep(sk) => { assert Inv(v'); }
+      case ReqSyncStep() => {
+        assert CrashTolerantMapSpecMod.NextStep(I(v), I(v'), uiop); // case boilerplate
+      }
+      case ReplySyncStep() => {
+        assert CrashTolerantMapSpecMod.NextStep(I(v), I(v'), uiop); // case boilerplate
+      }
+      case FreezeMapAdtStep() => {
+        assert CrashTolerantMapSpecMod.NextStep(I(v), I(v'), uiop); // case boilerplate
+      }
+      case CommitStartStep(seqBoundary) => {
+        assert CrashTolerantMapSpecMod.NextStep(I(v), I(v'), uiop); // case boilerplate
+      }
+      case CommitCompleteStep() => { CommitStepRefines(v, v', uiop, step); }
+      case CrashStep() => {
+        var stableLSN := v'.persistentImage.SeqEnd();
+        if v.ephemeral.Known? {
+          assert IPJ(v'.persistentImage.journal).DiscardRecent(stableLSN) == IEJ(v.ephemeral.journal).DiscardRecent(stableLSN); // trigger
+        }
+        assert CrashTolerantMapSpecMod.NextStep(I(v), I(v'), uiop); // case boilerplate
+      }
+    }
+    assert CrashTolerantMapSpecMod.Next(I(v), I(v'), uiop);
+  }
+}
+
